WIP implement LowParse.Steel.ArrayPtr

src/lowparse/LowParse.Steel.ArrayPtr.fst
@@ -1,770 +1,474 @@
 module LowParse.Steel.ArrayPtr
 
-module P = Steel.Pointer
-module SR = Steel.Reference
+module A = Steel.C.Array
+module R = Steel.Reference
 
-let array_prop (#a: Type) (ptr: P.t a) (x: A.array a) : Tot prop =
-  A.g_get_pointer x == ptr
+let g_is_null_from
+  (#base #t0: Type0)
+  (from: A.array_or_null_from base t0)
+: GTot bool
+= FStar.StrongExcludedMiddle.strong_excluded_middle (from == A.null_from base t0)
 
-let array (#a: Type) (ptr: P.t a) : Tot Type = (x: A.array a { array_prop ptr x })
-
-let t_array_t
-  (#a: Type)
-  (t_ptr: P.t a)
+inline_for_extraction
+noextract
+let array'
+  (#base #t0: Type0)
+  (from: A.array_or_null_from base t0)
 : Tot Type0
-= if P.g_is_null t_ptr then unit else SR.ghost_ref (array t_ptr)
+= (a: A.array base t0 { fst a == from })
 
-let t_perm_t
-  (#a: Type)
-  (t_ptr: P.t a)
-: Tot Type0
-= if P.g_is_null t_ptr then unit else SR.ghost_ref perm
+(* I could define t as follows:
+<<
+noeq
+type t
+  (base: Type0)
+  (t0: Type0)
+= {
+  from: A.array_or_null_from base t0;
+  to: Ghost.erased (if g_is_null_from from then unit else R.ghost_ref (array' from));
+}
+>>
+
+However, this dependent type does not extract to KReMLin very well (it is not inlined, etc.) Thus, instead, just like arrays, I can define t as a pair of an informative part and a ghost part, and move almost all dependency to the Ghost part, and express the remaining dependency between the informative part and the ghost part as a refinement:
+*)
 
 [@@erasable]
 noeq
-type tg (#a: Type) (t_ptr: P.t a) = {
-  t_array: t_array_t t_ptr;
-  t_perm: t_perm_t t_ptr;
+type t_nonnull
+  (base: Type0)
+  (t0: Type0)
+= {
+  from: A.array_or_null_from base t0;
+  to: R.ghost_ref (array' from);
 }
 
-noeq
-type t a = {
-  t_ptr: P.t a;
-  t_g: tg t_ptr;
-  t_prf: squash (P.g_is_null t_ptr == false ==> P.size_v (P.base_array_len (P.base t_ptr)) < 4294967296); // TODO: remove and switch to size_t
-}
+inline_for_extraction
+noextract
+let fst0 (#a #b: Type) (x: (a & b)) : Tot a = fst x
+inline_for_extraction
+noextract
+let snd0 (#a #b: Type) (x: (a & b)) : Tot b = snd x
 
-let null a = {
-  t_ptr = P.null a;
-  t_g = { t_array = (); t_perm = (); };
-  t_prf = ();
-}
+let t_prop
+  (#base #t0: Type0)
+  (x: (A.array_or_null_from base t0 & Ghost.erased (option (t_nonnull base t0))))
+: Tot prop
+= g_is_null_from (fst0 x) == None? (snd0 x) /\
+  (Some? (snd0 x) ==> (Some?.v (snd0 x)).from == fst0 x)
 
-let g_is_null x = P.g_is_null x.t_ptr
+let t base t0 =
+  (x: (A.array_or_null_from base t0 & Ghost.erased (option (t_nonnull base t0))) { t_prop x })
+
+let null base t0 = (A.null_from base t0, Ghost.hide None)
+
+let g_is_null x =
+  g_is_null_from (fst0 x)
+
+let array base t = A.array base t
+
+let len x = A.len x
 
 let varrayptr0_refine
-  (#a: Type)
-  (x: t a)
+  (#base #a: Type)
+  (x: t base a)
   (_: t_of emp)
 : Tot prop
 = g_is_null x == false
 
-let varrayptr0_payload2
-  (#a: Type)
-  (x: t a)
+[@@__steel_reduce__]
+let varrayptr0_dep_inner
+  (#base #a: Type)
+  (x: t base a)
   (_: t_of (emp `vrefine` varrayptr0_refine x))
-  (arp: t_of (SR.ghost_vptr #(array x.t_ptr) x.t_g.t_array `star` SR.ghost_vptr #perm x.t_g.t_perm))
+  (ar: normal (t_of (R.ghost_vptr (Some?.v (snd0 x)).to)))
 : Tot vprop
-= let (ar, p) = arp in
-  A.varrayp #a ar p
+= A.varray ar
 
-[@@__steel_reduce__] // to automatically reduce t_of, necessary for the call to normal below
-let varrayptr0_payload1
-  (#a: Type)
-  (x: t a)
-  (y: t_of (emp `vrefine` varrayptr0_refine x))
+[@@__steel_reduce__]
+let varrayptr0_dep_outer
+  (#base #a: Type)
+  (x: t base a)
+  (q: t_of (emp `vrefine` varrayptr0_refine x))
 : Tot vprop
-= (SR.ghost_vptr #(array x.t_ptr) x.t_g.t_array `star` SR.ghost_vptr #perm x.t_g.t_perm) `vdep` varrayptr0_payload2 x y
+= R.ghost_vptr (Some?.v (snd0 x)).to `vdep` varrayptr0_dep_inner x q
 
 let varrayptr0_rewrite
-  (#a: Type)
-  (x: t a)
-  (y: normal (t_of (emp `vrefine` varrayptr0_refine x `vdep` varrayptr0_payload1 x)))
-: GTot (v a)
-= let (| _, (| (ar, p), w |) |) = y in
-  A.length_get_pointer ar;
-  {
-    array = ar;
-    contents = w;
-    perm = p;
-    prf = ();
-  }
+  (#base #a: Type)
+  (x: t base a)
+  (res: normal (t_of (emp `vrefine` varrayptr0_refine x `vdep` varrayptr0_dep_outer x)))
+: Tot (v base a)
+= let (| _, (| ar, co |) |) = res in
+  { array = ar; contents = co; }
 
+[@@__steel_reduce__]
 let varrayptr0
-  (#a: Type)
-  (x: t a)
+  (#base #a: Type)
+  (x: t base a)
 : Tot vprop
-= emp `vrefine` varrayptr0_refine x `vdep` varrayptr0_payload1 x `vrewrite` varrayptr0_rewrite x
+= emp `vrefine` varrayptr0_refine x
+    `vdep` varrayptr0_dep_outer x
+    `vrewrite` varrayptr0_rewrite x
 
+val intro_varrayptr0
+  (#opened: _)
+  (#base #a: Type)
+  (x: t base a)
+  (ar: A.array base a)
+  (sq: squash (g_is_null x == false))
+: SteelGhost unit opened
+    (R.ghost_vptr (Some?.v (snd0 x)).to `star` A.varray ar)
+    (fun _ -> varrayptr0 x)
+    (requires (fun h ->
+      h (R.ghost_vptr (Some?.v (snd0 x)).to) == ar
+    ))
+    (ensures (fun h _ h' ->
+      let res = h' (varrayptr0 x) in
+      res.array == ar /\
+      res.contents == h (A.varray ar)
+    ))
+
+let intro_varrayptr0
+  x ar sq
+=
+  intro_vrefine emp (varrayptr0_refine x);
+  let q = gget (emp `vrefine` varrayptr0_refine x) in
+  intro_vdep
+    (R.ghost_vptr (Some?.v (snd0 x)).to)
+    (A.varray ar)
+    (varrayptr0_dep_inner x q);
+  intro_vdep
+    (emp `vrefine` varrayptr0_refine x)
+    (R.ghost_vptr (Some?.v (snd0 x)).to `vdep` varrayptr0_dep_inner x q)
+    (varrayptr0_dep_outer x);
+  intro_vrewrite
+    (emp `vrefine` varrayptr0_refine x `vdep` varrayptr0_dep_outer x)
+    (varrayptr0_rewrite x)
+
+val elim_varrayptr0
+  (#opened: _)
+  (#base #a: Type)
+  (x: t base a)
+: SteelGhost (Ghost.erased (R.ghost_ref (array' (fst0 x)) & A.array base a)) opened
+    (varrayptr0 x)
+    (fun res -> R.ghost_vptr (fst0 res) `star` A.varray (snd0 res))
+    (requires (fun _ -> True))
+    (ensures (fun h res h' ->
+      let pres = h (varrayptr0 x) in
+      let ar = snd0 res in
+      g_is_null x == false /\
+      fst0 res == (Some?.v (snd0 x)).to /\
+      pres.array == Ghost.reveal ar /\
+      h' (R.ghost_vptr (fst0 res)) == Ghost.reveal ar /\
+      h' (A.varray ar) == pres.contents
+    ))
+
+let elim_varrayptr0 x =
+  elim_vrewrite
+    (emp `vrefine` varrayptr0_refine x `vdep` varrayptr0_dep_outer x)
+    (varrayptr0_rewrite x);
+  let q = elim_vdep (emp `vrefine` varrayptr0_refine x) (varrayptr0_dep_outer x) in
+  elim_vrefine emp (varrayptr0_refine x);
+  change_equal_slprop
+    (varrayptr0_dep_outer x q)
+    (R.ghost_vptr (Some?.v (snd0 x)).to `vdep` varrayptr0_dep_inner x q);
+  let ar = elim_vdep (R.ghost_vptr (Some?.v (snd0 x)).to) (varrayptr0_dep_inner x q) in
+  let res = Ghost.hide ((Some?.v (snd0 x)).to, Ghost.reveal ar) in
+  change_equal_slprop
+    (R.ghost_vptr (Some?.v (snd0 x)).to)
+    (R.ghost_vptr (fst0 res));
+  change_equal_slprop
+    (varrayptr0_dep_inner x q ar)
+    (A.varray (snd0 res));
+  res
+  
 let is_arrayptr r = hp_of (varrayptr0 r)
-
 let arrayptr_sel r = sel_of (varrayptr0 r)
 
 val intro_varrayptr
   (#opened: _)
-  (#a: Type)
-  (x: t a)
-  (ga: SR.ghost_ref (array x.t_ptr))
-  (gp: SR.ghost_ref perm)
-  (a: array x.t_ptr)
-  (p: perm)
+  (#base #a: Type)
+  (x: t base a)
+  (ar: A.array base a)
+  (sq: squash (g_is_null x == false))
 : SteelGhost unit opened
-    (SR.ghost_vptr ga `star` SR.ghost_vptr gp `star` A.varrayp a p)
+    (R.ghost_vptr (Some?.v (snd0 x)).to `star` A.varray ar)
     (fun _ -> varrayptr x)
-    (fun h ->
-      P.g_is_null x.t_ptr == false /\
-      x.t_g.t_array == ga /\
-      x.t_g.t_perm == gp /\
-      can_be_split (SR.ghost_vptr ga `star` SR.ghost_vptr gp `star` A.varrayp a p) (SR.ghost_vptr ga) /\
-      can_be_split (SR.ghost_vptr ga `star` SR.ghost_vptr gp `star` A.varrayp a p) (SR.ghost_vptr gp) /\
-      h (SR.ghost_vptr ga) == a /\
-      h (SR.ghost_vptr gp) == p
-    )
-    (fun h _ h' ->
+    (requires (fun h ->
+      h (R.ghost_vptr (Some?.v (snd0 x)).to) == ar
+    ))
+    (ensures (fun h _ h' ->
       let res = h' (varrayptr x) in
-      res.array == a /\
-      res.contents == h (A.varrayp a p) /\
-      res.perm == p
-    )
-
-#push-options "--z3rlimit 32"
-#restart-solver
+      res.array == ar /\
+      res.contents == h (A.varray ar)
+    ))
 
 let intro_varrayptr
-  #_ #b x ga gp a p
+  x ar sq
 =
-  reveal_star_3 (SR.ghost_vptr ga) (SR.ghost_vptr gp) (A.varrayp a p);
-  let pa : squash (t_array_t x.t_ptr == SR.ghost_ref (array x.t_ptr)) = () in
-  let pp : squash (t_perm_t x.t_ptr == SR.ghost_ref perm) = () in
-  let a' : Ghost.erased (array x.t_ptr) = gget (SR.ghost_vptr ga) in
-  assert (Ghost.reveal a' == a);
-  let p' : Ghost.erased perm = gget (SR.ghost_vptr gp) in
-  assert (Ghost.reveal p' == p);
-  intro_vrefine emp (varrayptr0_refine x);
-  let y : Ghost.erased (t_of (emp `vrefine` varrayptr0_refine x)) = gget (emp `vrefine` varrayptr0_refine x) in
-  change_equal_slprop
-    (SR.ghost_vptr ga)
-    (SR.ghost_vptr #(array x.t_ptr) x.t_g.t_array);
-  change_equal_slprop
-    (SR.ghost_vptr gp)
-    (SR.ghost_vptr #perm x.t_g.t_perm);
-  SR.ghost_vptr #(array x.t_ptr) x.t_g.t_array `reveal_star` SR.ghost_vptr #perm x.t_g.t_perm;
-  intro_vdep
-    (SR.ghost_vptr #(array x.t_ptr) x.t_g.t_array `star` SR.ghost_vptr #perm x.t_g.t_perm)
-    (A.varrayp a p)
-    (varrayptr0_payload2 x y);
-  intro_vdep
-    (emp `vrefine` varrayptr0_refine x)
-    (SR.ghost_vptr #(array x.t_ptr) x.t_g.t_array `star` SR.ghost_vptr #perm x.t_g.t_perm `vdep` varrayptr0_payload2 x y)
-    (varrayptr0_payload1 x);
-  intro_vrewrite
-    (emp `vrefine` varrayptr0_refine x `vdep` varrayptr0_payload1 x)
-    (varrayptr0_rewrite x);
-  assert_norm (
-    emp `vrefine` varrayptr0_refine x `vdep` varrayptr0_payload1 x `vrewrite` varrayptr0_rewrite x ==
-    varrayptr0 x
-  );
-  change_equal_slprop
-    (emp `vrefine` varrayptr0_refine x `vdep` varrayptr0_payload1 x `vrewrite` varrayptr0_rewrite x)
-    (varrayptr0 x);
+  intro_varrayptr0 x ar sq;
   change_slprop_rel
     (varrayptr0 x)
     (varrayptr x)
     (fun u v -> u == v)
-    (fun _ -> ())
-
-#pop-options
-
-let intro_varrayptr'
-  (#opened: _)
-  (#b: Type)
-  (x: t b)
-  (x_ptr: P.t b)
-  (ga: SR.ghost_ref (array x_ptr))
-  (gp: SR.ghost_ref perm)
-  (a: array x_ptr)
-  (p: perm)
-: SteelGhost unit opened
-    (SR.ghost_vptr ga `star` SR.ghost_vptr gp `star` A.varrayp a p)
-    (fun _ -> varrayptr x)
-    (fun h ->
-      x_ptr == x.t_ptr /\
-      P.g_is_null x.t_ptr == false /\
-      x.t_g.t_array == ga /\
-      x.t_g.t_perm == gp /\
-      can_be_split (SR.ghost_vptr ga `star` SR.ghost_vptr gp `star` A.varrayp a p) (SR.ghost_vptr ga) /\
-      can_be_split (SR.ghost_vptr ga `star` SR.ghost_vptr gp `star` A.varrayp a p) (SR.ghost_vptr gp) /\
-      h (SR.ghost_vptr ga) == a /\
-      h (SR.ghost_vptr gp) == p
+    (fun m ->
+      assert_norm (hp_of (varrayptr x) == hp_of (varrayptr0 x));
+      assert_norm (sel_of (varrayptr x) m === sel_of (varrayptr0 x) m)
     )
-    (fun h _ h' ->
-      let res = h' (varrayptr x) in
-      res.array == a /\
-      res.contents == h (A.varrayp a p) /\
-      res.perm == p
-    )
-=
-  let ga' : SR.ghost_ref (array x.t_ptr) = ga in
-  change_equal_slprop
-    (SR.ghost_vptr ga)
-    (SR.ghost_vptr ga');
-  intro_varrayptr x ga' gp a p
-
-[@@erasable]
-noeq
-type elim_varrayptr_t
-  (#a: Type)
-  (ptr: P.t a)
-= {
-  e_g_array: SR.ghost_ref (array ptr);
-  e_g_perm: SR.ghost_ref perm;
-  e_array: array ptr;
-  e_perm: perm;
-}
 
 val elim_varrayptr
   (#opened: _)
-  (#a: Type)
-  (x: t a)
-: SteelGhost (elim_varrayptr_t x.t_ptr) opened
+  (#base #a: Type)
+  (x: t base a)
+: SteelGhost (Ghost.erased (R.ghost_ref (array' (fst0 x)) & A.array base a)) opened
     (varrayptr x)
-    (fun res -> SR.ghost_vptr res.e_g_array `star` SR.ghost_vptr res.e_g_perm `star` A.varrayp res.e_array res.e_perm)
-    (fun _ -> True)
-    (fun h res h' ->
-      let s = h (varrayptr x) in
-      P.g_is_null x.t_ptr == false /\
-      x.t_g.t_array == res.e_g_array /\
-      x.t_g.t_perm == res.e_g_perm /\
-      can_be_split (SR.ghost_vptr res.e_g_array `star` SR.ghost_vptr res.e_g_perm `star` A.varrayp res.e_array res.e_perm) (SR.ghost_vptr res.e_g_array) /\
-      can_be_split (SR.ghost_vptr res.e_g_array `star` SR.ghost_vptr res.e_g_perm `star` A.varrayp res.e_array res.e_perm) (SR.ghost_vptr res.e_g_perm) /\
-      h' (SR.ghost_vptr res.e_g_array) == res.e_array /\
-      h' (SR.ghost_vptr res.e_g_perm) == res.e_perm /\
-      s.array == res.e_array /\
-      s.perm == res.e_perm /\
-      h' (A.varrayp res.e_array res.e_perm) == s.contents
-    )
+    (fun res -> R.ghost_vptr (fst0 res) `star` A.varray (snd0 res))
+    (requires (fun _ -> True))
+    (ensures (fun h res h' ->
+      let pres = h (varrayptr x) in
+      let ar = snd0 res in
+      g_is_null x == false /\
+      fst0 res == (Some?.v (snd0 x)).to /\
+      pres.array == Ghost.reveal ar /\
+      h' (R.ghost_vptr (fst0 res)) == Ghost.reveal ar /\
+      h' (A.varray ar) == pres.contents
+    ))
 
 let elim_varrayptr
-  #_ #b x
+  #_ #base #a x
 =
   change_slprop_rel
     (varrayptr x)
     (varrayptr0 x)
     (fun u v -> u == v)
-    (fun _ -> ());
-  assert_norm (
-    emp `vrefine` varrayptr0_refine x `vdep` varrayptr0_payload1 x `vrewrite` varrayptr0_rewrite x ==
-    varrayptr0 x
-  );
-  change_equal_slprop
-    (varrayptr0 x)
-    (emp `vrefine` varrayptr0_refine x `vdep` varrayptr0_payload1 x `vrewrite` varrayptr0_rewrite x);
-  elim_vrewrite
-    (emp `vrefine` varrayptr0_refine x `vdep` varrayptr0_payload1 x)
-    (varrayptr0_rewrite x);
-  let y : Ghost.erased (t_of (emp `vrefine` varrayptr0_refine x)) = elim_vdep
-    (emp `vrefine` varrayptr0_refine x)
-    (varrayptr0_payload1 x)
-  in
-  elim_vrefine emp (varrayptr0_refine x);
-  let pa : squash (t_array_t x.t_ptr == SR.ghost_ref (array x.t_ptr)) = () in
-  let pp : squash (t_perm_t x.t_ptr == SR.ghost_ref perm) = () in
-  change_equal_slprop
-    (varrayptr0_payload1 x y)
-    (SR.ghost_vptr #(array x.t_ptr) x.t_g.t_array `star` SR.ghost_vptr #perm x.t_g.t_perm `vdep` varrayptr0_payload2 x y);
-  let gap : Ghost.erased (t_of (SR.ghost_vptr #(array x.t_ptr) x.t_g.t_array `star` SR.ghost_vptr #perm x.t_g.t_perm)) = elim_vdep
-    (SR.ghost_vptr #(array x.t_ptr) x.t_g.t_array `star` SR.ghost_vptr #perm x.t_g.t_perm)
-    (varrayptr0_payload2 x y)
-  in
-  SR.ghost_vptr #(array x.t_ptr) x.t_g.t_array `reveal_star` SR.ghost_vptr #perm x.t_g.t_perm;
-  let g_a : Ghost.erased (array x.t_ptr) = SR.ghost_read #(array x.t_ptr) x.t_g.t_array in
-  let a : array x.t_ptr = Ghost.reveal g_a in
-  let g_p : Ghost.erased perm = SR.ghost_read #perm x.t_g.t_perm in
-  let p : perm = Ghost.reveal g_p in
-  let res = {
-    e_g_array = x.t_g.t_array;
-    e_g_perm = x.t_g.t_perm;
-    e_array = a;
-    e_perm = p;
-  } in
-  change_equal_slprop
-    (SR.ghost_vptr #(array x.t_ptr) x.t_g.t_array)
-    (SR.ghost_vptr res.e_g_array);
-  change_equal_slprop
-    (SR.ghost_vptr #perm x.t_g.t_perm)
-    (SR.ghost_vptr res.e_g_perm);
-  change_equal_slprop
-    (varrayptr0_payload2 x y gap)
-    (A.varrayp res.e_array res.e_perm);
-  reveal_star_3 (SR.ghost_vptr res.e_g_array) (SR.ghost_vptr res.e_g_perm) (A.varrayp res.e_array res.e_perm);
-  res
+    (fun m ->
+      assert_norm (hp_of (varrayptr x) == hp_of (varrayptr0 x));
+      assert_norm (sel_of (varrayptr x) m === sel_of (varrayptr0 x) m)
+    );
+  elim_varrayptr0 x
 
 let varrayptr_not_null
   x
-= let res = elim_varrayptr x in
-  intro_varrayptr x res.e_g_array res.e_g_perm res.e_array res.e_perm
-
-[@@__steel_reduce__]
-let varrayptr_ghost_refs
-  (#a: Type)
-  (x: t a)
-: Tot vprop
-= if P.g_is_null x.t_ptr
-  then emp
-  else SR.ghost_vptr #(array x.t_ptr) x.t_g.t_array `star` SR.ghost_vptr #perm x.t_g.t_perm
-
-let varrayptr_ghost_refs_rewrite
-  (#a: Type)
-  (x: t a)
-  (r: t_of (varrayptr_ghost_refs x))
-: GTot (array x.t_ptr `P.gpair` perm)
 =
-  if P.g_is_null x.t_ptr
-  then
-    let _ = A.is_null_get_pointer (A.null a) in
-    A.null a `P.GPair` full_perm
-  else 
-    let r : (array x.t_ptr & perm) = r in
-    fst r `P.GPair` snd r
-
-[@@__steel_reduce__]
-let varrayptr_or_null_payload
-  (#a: Type)
-  (x: t a)
-  (r: (array x.t_ptr `P.gpair` perm))
-: Tot vprop
-= A.varrayp_or_null (P.GPair?.fst r) (P.GPair?.snd r)
-
-let varrayptr_or_null_rewrite
-  (#a: Type)
-  (x: t a)
-  (r: normal (t_of (varrayptr_ghost_refs x `vrewrite` varrayptr_ghost_refs_rewrite x `vdep` varrayptr_or_null_payload x)))
-: GTot (option (v a))
-= let (| P.GPair ar p, r |) = r in
-  match P.g_is_null x.t_ptr, r with
-  | false, Some r ->
-    A.length_get_pointer ar;
-    Some ({
-      array = ar;
-      contents = r;
-      perm = p;
-      prf = ();
-    })
-  | _ -> None
+  let tmp = elim_varrayptr x in
+  change_equal_slprop
+    (R.ghost_vptr (fst0 tmp))
+    (R.ghost_vptr (Some?.v (snd0 x)).to);
+  intro_varrayptr x (snd0 tmp) ()
 
 [@@__steel_reduce__]
 let varrayptr_or_null0
-  (#a: Type)
-  (x: t a)
+  (#base #a: Type)
+  (r: t base a)
 : Tot vprop
-= varrayptr_ghost_refs x `vrewrite` varrayptr_ghost_refs_rewrite x `vdep` varrayptr_or_null_payload x `vrewrite` varrayptr_or_null_rewrite x
+= if g_is_null r
+  then emp `vrewrite` (fun _ -> None <: option (v base a))
+  else varrayptr r `vrewrite` Some
 
 let is_arrayptr_or_null r = hp_of (varrayptr_or_null0 r)
+let arrayptr_or_null_sel r = sel_of (varrayptr_or_null0 r)
 
-let arrayptr_or_null_sel r = fun h -> sel_of (varrayptr_or_null0 r) h
-
-#set-options "--ide_id_info_off"
-
-let intro_varrayptr_or_null_none #_ #a x =
-  change_equal_slprop
-    emp
-    (varrayptr_ghost_refs x);
-  intro_vrewrite (varrayptr_ghost_refs x) (varrayptr_ghost_refs_rewrite x);
-  A.intro_varrayp_or_null_none (A.null a) full_perm;
-  intro_vdep
-    (varrayptr_ghost_refs x `vrewrite` varrayptr_ghost_refs_rewrite x)
-    (A.varrayp_or_null (A.null a) full_perm)
-    (varrayptr_or_null_payload x);
-  intro_vrewrite (varrayptr_ghost_refs x `vrewrite` varrayptr_ghost_refs_rewrite x `vdep` varrayptr_or_null_payload x) (varrayptr_or_null_rewrite x);
-  change_equal_slprop
-    (varrayptr_ghost_refs x `vrewrite` varrayptr_ghost_refs_rewrite x `vdep` varrayptr_or_null_payload x `vrewrite` varrayptr_or_null_rewrite x)
-    (varrayptr_or_null0 x);
-  change_slprop_rel
-    (varrayptr_or_null0 x)
-    (varrayptr_or_null x)
-    (fun u v -> u == v)
-    (fun h ->
-      assert_norm (hp_of (varrayptr_or_null0 x) == hp_of (varrayptr_or_null x));
-      assert_norm (sel_of (varrayptr_or_null0 x) h === sel_of (varrayptr_or_null x) h)
-    )
-
-let intro_varrayptr_or_null_some #_ #a x =
-  let r = elim_varrayptr x in
-  reveal_star (SR.ghost_vptr r.e_g_array) (SR.ghost_vptr r.e_g_perm);
-  change_equal_slprop
-    (SR.ghost_vptr r.e_g_array `star` SR.ghost_vptr r.e_g_perm)
-    (varrayptr_ghost_refs x);
-  intro_vrewrite (varrayptr_ghost_refs x) (varrayptr_ghost_refs_rewrite x);
-  A.intro_varrayp_or_null_some r.e_array r.e_perm;
-  intro_vdep
-    (varrayptr_ghost_refs x `vrewrite` varrayptr_ghost_refs_rewrite x)
-    (A.varrayp_or_null r.e_array r.e_perm)
-    (varrayptr_or_null_payload x);
-  intro_vrewrite (varrayptr_ghost_refs x `vrewrite` varrayptr_ghost_refs_rewrite x `vdep` varrayptr_or_null_payload x) (varrayptr_or_null_rewrite x);
-  change_equal_slprop
-    (varrayptr_ghost_refs x `vrewrite` varrayptr_ghost_refs_rewrite x `vdep` varrayptr_or_null_payload x `vrewrite` varrayptr_or_null_rewrite x)
-    (varrayptr_or_null0 x);
-  change_slprop_rel
-    (varrayptr_or_null0 x)
-    (varrayptr_or_null x)
-    (fun u v -> u == v)
-    (fun h ->
-      assert_norm (hp_of (varrayptr_or_null0 x) == hp_of (varrayptr_or_null x));
-      assert_norm (sel_of (varrayptr_or_null0 x) h === sel_of (varrayptr_or_null x) h)
-    )
-
-val intro_varrayptr_or_null
-  (#opened: _)
-  (#b: Type)
-  (x: P.t b)
-  (a: array x)
-  (p: perm)
-: SteelGhost (Ghost.erased (t b)) opened
-    (A.varrayp_or_null a p)
-    (fun res -> varrayptr_or_null res)
-    (fun _ -> 
-      P.g_is_null x == false ==> P.size_v (P.base_array_len (P.base x)) < 4294967296 // TODO: remove and switch to size_t
-    )
-    (fun h res h' ->
-      res.t_ptr == x /\
-      begin match P.g_is_null x, h (A.varrayp_or_null a p), h' (varrayptr_or_null res) with
-      | true, None, None -> True
-      | false, Some s, Some r ->
-        r.array == a /\
-        r.perm == p /\
-        r.contents == s
-      | _ -> False    
-      end
-    )
-
-let intro_varrayptr_or_null
-  #_ #b x a p
+let intro_varrayptr_or_null_none
+  #_ #base #a x
 =
-  A.is_null_get_pointer a;
-  if P.g_is_null x
-  then begin
-    A.assert_null a _;
-    let res : Ghost.erased (t b) = Ghost.hide (null _) in
-    intro_varrayptr_or_null_none res;
-    res
-  end else begin
-    A.assert_not_null a _;
-    let ga : SR.ghost_ref (array x) = SR.ghost_alloc a in
-    let gp : SR.ghost_ref perm = SR.ghost_alloc p in
-    let res : Ghost.erased (t b) = Ghost.hide ({
-      t_ptr = x;
-      t_g = {
-        t_array = ga;
-        t_perm = gp;
-      };
-      t_prf = ();
-    }) in
-    reveal_star_3 (SR.ghost_vptr ga) (SR.ghost_vptr gp) (A.varrayp a p);
-    intro_varrayptr' res x ga gp a p;
-    intro_varrayptr_or_null_some res;
-    res
-  end
-
-unfold
-let coerce (#a: Type) (x: a) (b: Type) : Pure b (requires (a == b)) (ensures (fun y -> a == b /\ x == y)) = x
-
-unfold
-let coerce2 (#a: Type) (x: a) (b: Type) (sq: squash (a == b)) : Tot b = x
-
-let elim_varrayptr_or_null_some #_ #a x =
+  intro_vrewrite emp (fun _ -> None <: option (v base a));
   change_slprop_rel
+    (emp `vrewrite` (fun _ -> None <: option (v base a)))
     (varrayptr_or_null x)
-    (varrayptr_or_null0 x)
     (fun u v -> u == v)
-    (fun h ->
-      assert_norm (hp_of (varrayptr_or_null0 x) == hp_of (varrayptr_or_null x));
-      assert_norm (sel_of (varrayptr_or_null0 x) h === sel_of (varrayptr_or_null x) h)
-    );
-  elim_vrewrite
-    (varrayptr_ghost_refs x `vrewrite` varrayptr_ghost_refs_rewrite x `vdep` varrayptr_or_null_payload x) (varrayptr_or_null_rewrite x);
-  let _ : squash (P.g_is_null x.t_ptr == false) = () in
-  let pa : squash (t_array_t x.t_ptr == SR.ghost_ref (array x.t_ptr)) = () in
-  let pp : squash (t_perm_t x.t_ptr == SR.ghost_ref perm) = () in
-  let ga : SR.ghost_ref (array x.t_ptr) = coerce2 x.t_g.t_array (SR.ghost_ref (array x.t_ptr)) pa in
-  let gp : SR.ghost_ref perm = coerce2 x.t_g.t_perm (SR.ghost_ref perm) pp in
-  let g : Ghost.erased (P.gpair (array x.t_ptr) perm) = elim_vdep
-    (varrayptr_ghost_refs x `vrewrite` varrayptr_ghost_refs_rewrite x)
-    (varrayptr_or_null_payload x)
-  in
-  elim_vrewrite (varrayptr_ghost_refs x) (varrayptr_ghost_refs_rewrite x);
-  change_equal_slprop
-    (varrayptr_ghost_refs x)
-    (SR.ghost_vptr ga `star` SR.ghost_vptr gp);
-  SR.ghost_vptr ga `reveal_star` SR.ghost_vptr gp;
-  A.is_null_get_pointer (P.GPair?.fst g);
-  change_equal_slprop
-    (varrayptr_or_null_payload x g)
-    (A.varrayp_or_null (P.GPair?.fst g) (P.GPair?.snd g));
-  A.assert_not_null (P.GPair?.fst g) (P.GPair?.snd g);
-  reveal_star_3 (SR.ghost_vptr ga) (SR.ghost_vptr gp) (A.varrayp (P.GPair?.fst g) (P.GPair?.snd g));
-  intro_varrayptr x ga gp (P.GPair?.fst g) (P.GPair?.snd g)
+    (fun _ -> ())
 
-let elim_varrayptr_or_null_none #_ #a x =
+let intro_varrayptr_or_null_some
+  #_ #base #a x
+=
+  intro_vrewrite (varrayptr x) Some;
   change_slprop_rel
+    (varrayptr x `vrewrite` Some)
     (varrayptr_or_null x)
-    (varrayptr_or_null0 x)
     (fun u v -> u == v)
-    (fun h ->
-      assert_norm (hp_of (varrayptr_or_null0 x) == hp_of (varrayptr_or_null x));
-      assert_norm (sel_of (varrayptr_or_null0 x) h === sel_of (varrayptr_or_null x) h)
-    );
-  elim_vrewrite
-    (varrayptr_ghost_refs x `vrewrite` varrayptr_ghost_refs_rewrite x `vdep` varrayptr_or_null_payload x) (varrayptr_or_null_rewrite x);
-  let g : Ghost.erased (P.gpair (array x.t_ptr) perm) = elim_vdep
-    (varrayptr_ghost_refs x `vrewrite` varrayptr_ghost_refs_rewrite x)
-    (varrayptr_or_null_payload x)
-  in
-  change_equal_slprop
-    (varrayptr_or_null_payload x g)
-    (A.varrayp_or_null (P.GPair?.fst g) (P.GPair?.snd g));
-  A.is_null_get_pointer (P.GPair?.fst g);
-  if P.g_is_null x.t_ptr
+    (fun _ -> ())
+
+let elim_varrayptr_or_null_some
+  #_ #base #a x
+=
+  if g_is_null x
   then begin
-    A.assert_null (P.GPair?.fst g) (P.GPair?.snd g);
-    elim_vrewrite (varrayptr_ghost_refs x) (varrayptr_ghost_refs_rewrite x);
-    change_equal_slprop
-      (varrayptr_ghost_refs x)
-      emp
-  end else begin
-    A.assert_not_null (P.GPair?.fst g) (P.GPair?.snd g);
-    assert False;
     change_slprop_rel
-      ((varrayptr_ghost_refs x `vrewrite` varrayptr_ghost_refs_rewrite x) `star` A.varrayp (P.GPair?.fst g) (P.GPair?.snd g))
+      (varrayptr_or_null x)
+      (emp `vrewrite` (fun _ -> None <: option (v base a)))
+      (fun u v -> u == v)
+      (fun _ -> ());
+    elim_vrewrite
       emp
-      (fun _ _ -> False)
-      (fun _ -> ())
+      (fun _ -> None <: option (v base a));
+    assert False;
+    change_equal_slprop
+      emp
+      (varrayptr x)
+  end else begin
+    change_slprop_rel
+      (varrayptr_or_null x)
+      (varrayptr x `vrewrite` Some)
+      (fun u v -> u == v)
+      (fun _ -> ());
+    elim_vrewrite (varrayptr x) Some
   end
 
-let is_null_none
-  (#opened: _)
+let elim_varrayptr_or_null_none
+  #_ #base #a x
+=
+  if g_is_null x
+  then begin
+    change_slprop_rel
+      (varrayptr_or_null x)
+      (emp `vrewrite` (fun _ -> None <: option (v base a)))
+      (fun u v -> u == v)
+      (fun _ -> ());
+    elim_vrewrite
+      emp
+      (fun _ -> None <: option (v base a))
+  end else begin
+    change_slprop_rel
+      (varrayptr_or_null x)
+      (varrayptr x `vrewrite` Some)
+      (fun u v -> u == v)
+      (fun _ -> ());
+    elim_vrewrite (varrayptr x) Some;
+    assert False;
+    change_equal_slprop
+      (varrayptr x)
+      emp
+  end
+
+let ghost_vptr_or_none
   (#a: Type)
-  (x: t a)
-: SteelGhost unit opened
+  (r: option (R.ghost_ref a))
+: Tot vprop
+= if None? r
+  then emp
+  else R.ghost_vptr (Some?.v r)
+
+let array_or_null_of_intro
+  (#opened: _)
+  (#base #a: Type)
+  (x: t base a)
+: SteelGhost (Ghost.erased (A.array_or_null base a & option (R.ghost_ref (array' (fst0 x))))) opened
     (varrayptr_or_null x)
-    (fun _ -> varrayptr_or_null x)
+    (fun res -> A.varray_or_null (fst0 res) `star` ghost_vptr_or_none (snd0 res))
     (fun _ -> True)
-    (fun h _ h' ->
-      let s = h (varrayptr_or_null x) in
-      h' (varrayptr_or_null x) == s /\
-      g_is_null x == None? s
+    (fun h res h' ->
+      let z : option (v base a) = h (varrayptr_or_null x) in
+      fst0 (fst0 res) == fst0 x /\
+      (None? z <==> g_is_null x) /\
+      (None? z <==> A.g_is_null (fst0 res)) /\
+      (None? z <==> None? (snd0 res)) /\
+      (Some? z ==> (
+        Some?.v (snd0 res) == (Some?.v (snd0 x)).to /\
+        (h' (R.ghost_vptr (Some?.v (snd0 res))) <: A.array_or_null base a) == fst0 res /\
+        (Some?.v z).array == fst0 res /\
+        (Some?.v z).contents == h' (A.varray (fst0 res))
+      ))
     )
 =
   if g_is_null x
   then begin
     elim_varrayptr_or_null_none x;
-    intro_varrayptr_or_null_none x
+    let res = (A.null base a, None) in
+    change_equal_slprop
+      emp
+      (A.varray_or_null (fst0 res));
+    change_equal_slprop
+      emp
+      (ghost_vptr_or_none (snd0 res));
+    res
   end else begin
     elim_varrayptr_or_null_some x;
+    let tmp = elim_varrayptr x in
+    let res = (snd0 tmp, Some (fst0 tmp)) in
+    change_equal_slprop
+      (R.ghost_vptr (fst0 tmp))
+      (ghost_vptr_or_none (snd0 res));
+    change_equal_slprop
+      (A.varray (snd0 tmp))
+      (A.varray_or_null (fst0 res));
+    res
+  end
+
+let array_or_null_of_elim
+  (#opened: _)
+  (#base #a: Type)
+  (x: t base a)
+  (res: Ghost.erased (A.array_or_null base a & option (R.ghost_ref (array' (fst0 x)))))
+: SteelGhost unit opened
+    (A.varray_or_null (fst0 res) `star` ghost_vptr_or_none (snd0 res))
+    (fun _ -> varrayptr_or_null x)
+    (fun h ->
+      fst0 (fst0 res) == fst0 x /\
+      (g_is_null x <==> A.g_is_null (fst0 res)) /\
+      (g_is_null x <==> None? (snd0 res)) /\
+      (Some? (snd0 res) ==> (
+        Some?.v (snd0 res) == (Some?.v (snd0 x)).to /\
+        (h (R.ghost_vptr (Some?.v (snd0 res))) <: A.array_or_null base a) == fst0 res
+      ))
+    )
+    (fun h _ h' ->
+      let z : option (v base a) = h' (varrayptr_or_null x) in
+      fst0 (fst0 res) == fst0 x /\
+      (None? z <==> g_is_null x) /\
+      (None? z <==> A.g_is_null (fst0 res)) /\
+      (None? z <==> None? (snd0 res)) /\
+      (Some? z ==> (
+        (h (R.ghost_vptr (Some?.v (snd0 res))) <: A.array_or_null base a) == fst0 res /\
+        (Some?.v z).array == fst0 res /\
+        (Some?.v z).contents == h (A.varray (fst0 res))
+      ))
+    )
+= if g_is_null x
+  then begin
+    change_equal_slprop
+      (A.varray_or_null (fst0 res))
+      emp;
+    change_equal_slprop
+      (ghost_vptr_or_none (snd0 res))
+      emp;
+    intro_varrayptr_or_null_none x
+  end else begin
+    let ar : A.array base a = fst0 res in
+    change_equal_slprop
+      (A.varray_or_null (fst0 res))
+      (A.varray ar);
+    change_equal_slprop
+      (ghost_vptr_or_none (snd0 res))
+      (R.ghost_vptr (Some?.v (snd0 x)).to);
+    intro_varrayptr x ar ();
     intro_varrayptr_or_null_some x
   end
 
-let is_null
-  #_ #a x
+let is_null #base #a x
 =
-  is_null_none x;
-  change_slprop_rel
-    (varrayptr_or_null x)
-    (varrayptr_or_null0 x)
-    (fun u v -> u == v)
-    (fun h ->
-      assert_norm (hp_of (varrayptr_or_null0 x) == hp_of (varrayptr_or_null x));
-      assert_norm (sel_of (varrayptr_or_null0 x) h === sel_of (varrayptr_or_null x) h)
-    );
-  elim_vrewrite
-    (varrayptr_ghost_refs x `vrewrite` varrayptr_ghost_refs_rewrite x `vdep` varrayptr_or_null_payload x) (varrayptr_or_null_rewrite x);
-  let g : Ghost.erased (P.gpair (array x.t_ptr) perm) = elim_vdep
-    (varrayptr_ghost_refs x `vrewrite` varrayptr_ghost_refs_rewrite x)
-    (varrayptr_or_null_payload x)
+  let tmp = array_or_null_of_intro x in
+  let ar : (ar: A.array_or_null base a { ar == fst0 tmp }) =
+    (fst0 x, snd0 (fst0 tmp))
   in
   change_equal_slprop
-    (varrayptr_or_null_payload x g)
-    (A.varrayp_or_null (Ghost.reveal (Ghost.hide (P.GPair?.fst g))) (P.GPair?.snd g));
-  let ar = A.reveal x.t_ptr (Ghost.hide (P.GPair?.fst g)) (P.GPair?.snd g) in
-  A.is_null_get_pointer ar;
-  let res = A.is_null ar _ in
-  intro_vdep
-    (varrayptr_ghost_refs x `vrewrite` varrayptr_ghost_refs_rewrite x)
-    (A.varrayp_or_null ar (P.GPair?.snd g))
-    (varrayptr_or_null_payload x);
-  intro_vrewrite
-    (varrayptr_ghost_refs x `vrewrite` varrayptr_ghost_refs_rewrite x `vdep` varrayptr_or_null_payload x) (varrayptr_or_null_rewrite x);
-  change_slprop_rel
-    (varrayptr_or_null0 x)
-    (varrayptr_or_null x)
-    (fun u v -> u == v)
-    (fun h ->
-      assert_norm (hp_of (varrayptr_or_null0 x) == hp_of (varrayptr_or_null x));
-      assert_norm (sel_of (varrayptr_or_null0 x) h === sel_of (varrayptr_or_null x) h)
-    );
+     (A.varray_or_null (fst0 tmp))
+     (A.varray_or_null ar);
+  let res = A.is_null ar in
+  change_equal_slprop
+    (A.varray_or_null ar)
+    (A.varray_or_null (fst0 tmp));
+  array_or_null_of_elim x tmp;
   return res
+
+let adjacent x1 x2 = A.adjacent x1 x2
+let merge x1 x2 = A.merge x1 x2
 
 let join al ar =
-  let el = elim_varrayptr al in
-  let er = elim_varrayptr ar in
-  SR.ghost_free er.e_g_array;
-  SR.ghost_free er.e_g_perm;
+  let tmpr = elim_varrayptr ar in
+  R.ghost_free (fst0 tmpr);
+  let tmpl = elim_varrayptr al in
+  let res = A.join' (snd0 tmpl) (snd0 tmpr) in
+  R.ghost_write (fst0 tmpl) (Ghost.reveal res);
   change_equal_slprop
-    (A.varrayp er.e_array er.e_perm)
-    (A.varrayp er.e_array el.e_perm);
-  let a' = A.join' el.e_array er.e_array _ in
-  A.length_get_pointer a';
-  A.get_pointer_merge el.e_array er.e_array;
-  SR.ghost_write el.e_g_array (Ghost.reveal a');
-  reveal_star_3 (SR.ghost_vptr el.e_g_array) (SR.ghost_vptr el.e_g_perm) (A.varrayp a' el.e_perm);
-  intro_varrayptr al el.e_g_array el.e_g_perm a' el.e_perm
-
-let split x i =
-  varrayptr_not_null x;
-  let e = elim_varrayptr x in
-  change_equal_slprop
-    (A.varrayp e.e_array e.e_perm)
-    (A.varrayp (Ghost.hide e.e_array) e.e_perm);
-  A.intro_varrayp_or_null_some (Ghost.hide e.e_array) e.e_perm;
-  let a = A.reveal x.t_ptr (Ghost.hide e.e_array) _ in
-  A.assert_not_null a e.e_perm;
-  let j = P.mk_size_t i in
-  let alar = A.splitp a _ j in
-  A.get_pointer_gsplit a j;
-  SR.ghost_write e.e_g_array (fst alar);
-  reveal_star_3 (SR.ghost_vptr e.e_g_array) (SR.ghost_vptr e.e_g_perm) (A.varrayp (fst alar) e.e_perm);
-  intro_varrayptr x e.e_g_array e.e_g_perm (fst alar) e.e_perm;
-  let ar = snd alar in
-  change_equal_slprop
-    (A.varrayp (snd alar) e.e_perm)
-    (A.varrayp ar e.e_perm);
-  A.intro_varrayp_or_null_some ar _;
-  let pr = A.get_pointer ar _ in
-  A.assert_not_null ar _;
-  let ga : SR.ghost_ref (array pr) = SR.ghost_alloc ar in
-  let gp : SR.ghost_ref perm = SR.ghost_alloc e.e_perm in
-  let res = ({
-    t_ptr = pr;
-    t_g = {
-      t_array = ga;
-      t_perm = gp;
-    };
-    t_prf = ();
-  }) in
-  reveal_star_3 (SR.ghost_vptr ga) (SR.ghost_vptr gp) (A.varrayp ar e.e_perm);
-  intro_varrayptr' res pr ga gp ar e.e_perm;
-  return res
-
-let alloc x n =
-  let ar = A.malloc x (P.mk_size_t n) in
-  let p = A.get_pointer ar _ in
-  A.is_null_get_pointer ar;
-  A.length_get_pointer ar;
-  let g = intro_varrayptr_or_null p ar _ in
-  let res = {
-    t_ptr = p;
-    t_g = g.t_g;
-    t_prf = g.t_prf;
-  } in
-  change_equal_slprop
-    (varrayptr_or_null g)
-    (varrayptr_or_null res);
-  return res
-
-let index #b r i =
-  let e = elim_varrayptr r in
-  let g : Ghost.erased (A.array b) = Ghost.hide e.e_array in
-  change_equal_slprop
-    (A.varrayp e.e_array e.e_perm)
-    (A.varrayp g e.e_perm);
-  A.intro_varrayp_or_null_some g _;
-  let a = A.reveal r.t_ptr g _ in
-  A.assert_not_null a _;
-  let res = A.indexp a _ (P.mk_size_t i) in
-  intro_varrayptr r e.e_g_array e.e_g_perm a _;
-  return res
-
-let upd #b r i v =
-  let e = elim_varrayptr r in
-  let g : Ghost.erased (A.array b) = Ghost.hide e.e_array in
-  change_equal_slprop
-    (A.varrayp e.e_array e.e_perm)
-    (A.varray g);
-  A.intro_varrayp_or_null_some g _;
-  let a = A.reveal r.t_ptr g _ in
-  A.assert_not_null a _;
-  A.upd a (P.mk_size_t i) v;
-  intro_varrayptr r e.e_g_array e.e_g_perm a _
-
-let free r =
-  let e = elim_varrayptr r in
-  SR.ghost_free e.e_g_array;
-  SR.ghost_free e.e_g_perm;
-  let g : Ghost.erased (A.array _) = Ghost.hide e.e_array in
-  change_equal_slprop
-    (A.varrayp e.e_array e.e_perm)
-    (A.varray g);
-  A.intro_varrayp_or_null_some g _;
-  let a = A.reveal r.t_ptr g _ in
-  A.assert_not_null a _;
-  A.free a
-
-let share r =
-  let e = elim_varrayptr r in
-  let p = A.share e.e_array _ in
-  SR.ghost_write e.e_g_perm p;
-  reveal_star_3 (SR.ghost_vptr e.e_g_array) (SR.ghost_vptr e.e_g_perm) (A.varrayp e.e_array p);
-  intro_varrayptr r e.e_g_array e.e_g_perm e.e_array p;
-  let ga : SR.ghost_ref (array r.t_ptr) = SR.ghost_alloc e.e_array in
-  let gp : SR.ghost_ref perm = SR.ghost_alloc p in
-  let res = {
-    t_ptr = r.t_ptr;
-    t_g = {
-      t_array = ga;
-      t_perm = gp;
-    };
-    t_prf = ();
-  } in
-  reveal_star_3 (SR.ghost_vptr ga) (SR.ghost_vptr gp) (A.varrayp e.e_array p);
-  intro_varrayptr' res r.t_ptr ga gp e.e_array p;
-  return res
-
-let gather r1 r2 =
-  let e1 = elim_varrayptr r1 in
-  let e2 = elim_varrayptr r2 in
-  SR.ghost_free e2.e_g_array;
-  SR.ghost_free e2.e_g_perm;
-  assert (e2.e_array == e1.e_array);
-  change_equal_slprop
-    (A.varrayp e2.e_array e2.e_perm)
-    (A.varrayp e1.e_array e2.e_perm);
-  let p = A.gather e1.e_array e1.e_perm e2.e_perm in
-  SR.ghost_write e1.e_g_perm p;
-  reveal_star_3 (SR.ghost_vptr e1.e_g_array) (SR.ghost_vptr e1.e_g_perm) (A.varrayp e1.e_array p);
-  intro_varrayptr r1 e1.e_g_array e1.e_g_perm e1.e_array p
-
-let enter x p =
-  A.intro_varrayp_or_null_some x _;
-  let pt = A.get_pointer x _ in
-  A.assert_not_null x _;
-  A.is_null_get_pointer x;
-  A.length_get_pointer x;
-  let ga : SR.ghost_ref (array pt) = SR.ghost_alloc x in
-  let gp : SR.ghost_ref perm = SR.ghost_alloc p in
-  let res = {
-    t_ptr = pt;
-    t_g = {
-      t_array = ga;
-      t_perm = gp;
-    };
-    t_prf = ();
-  } in
-  reveal_star_3 (SR.ghost_vptr ga) (SR.ghost_vptr gp) (A.varrayp x p);
-  intro_varrayptr' res pt ga gp x p;
-  return res
-
-let exit x =
-  let e = elim_varrayptr x in
-  reveal_star_3 (SR.ghost_vptr e.e_g_array) (SR.ghost_vptr e.e_g_perm) (A.varrayp e.e_array e.e_perm);
-  SR.ghost_free e.e_g_array;
-  SR.ghost_free e.e_g_perm;
-  change_equal_slprop
-    (A.varrayp e.e_array e.e_perm)
-    (A.varrayp (Ghost.hide e.e_array) e.e_perm);
-  A.intro_varrayp_or_null_some (Ghost.hide e.e_array) e.e_perm;
-  let a = A.reveal x.t_ptr (Ghost.hide e.e_array) _ in
-  A.assert_not_null a e.e_perm;
-  let res = (a, e.e_perm) in
-  change_equal_slprop
-    (A.varrayp a e.e_perm)
-    (A.varrayp (fst res) (snd res));
-  return res
+    (R.ghost_vptr (fst0 tmpl))
+    (R.ghost_vptr (Some?.v (snd0 al)).to);
+  intro_varrayptr al res ()
